Towards variables.

LambdaS5/coq/LjsInitEnv.v
@@ -1929,8 +1929,7 @@ expr_if (expr_op2 binary_op_stx_eq (expr_id "context") expr_null)
 .
 Definition ex_privEnvGet := 
 expr_if (expr_op2 binary_op_stx_eq (expr_id "context") expr_null)
-(expr_if (expr_id "strict") (expr_app (expr_id "%UnboundId") [expr_id "id"])
- expr_undefined)
+(expr_app (expr_id "%UnboundId") [expr_id "id"])
 (expr_if
  (expr_op2 binary_op_stx_eq
   (expr_get_obj_attr oattr_class (expr_id "context"))
